**Question:**


Consider the context-free grammar
`S -> S S + | S S * | a`

Show how the string `aa+a*` can be generated by this grammar:

**Answer:**

Start symbol     = `S`
Terminal symbols = `{+,*,a}`
Production rules =

```
S -> S S *
  -> S a *
  -> S S + a *
  -> S a + a *
  -> a a + a *
```

Explanation:

You start with `S -> S S *` as defined in the question. Then you replace the
second `S` with `a` to satisfy `a*`. After that you replace `S` with `S S +` as
defined in the question, which gets you `S S + a *`. Then replace each remaining `S`
with `a`.

Another way:

```
S -> S S *
  -> S S + S *
  -> a S + S *
  -> a a + S *
  -> a a + a *
```

This expands first before filling in the `a`.

---

**Question:**

Construct a parse tree for this string.

**Answer:**

```
          S
         /|\
       /  |  \
     /    |    \
    S     S     *
  / | \   |
 S  S  +  a
 |  |
 a  a
```
